Semantic/Fsub/Soundness.lean
@@ -8,8 +8,12 @@ theorem sem_typ_var :
   constructor; constructor
   apply And.intro Reduce.red_refl _
   cases x
-  case bound bx => rfl
-  case free fx => rfl
+  case bound bx =>
+    simp [Ty.val_denot]
+    rfl
+  case free fx =>
+    simp [Ty.val_denot]
+    rfl
 
 theorem sem_typ_abs
   (ht : (Γ,x:T1) ⊨ e : T2) :
@@ -20,17 +24,53 @@ theorem sem_typ_abs
   apply And.intro Reduce.red_refl _
   simp [Ty.val_denot]
   constructor; constructor
-  split_ands
+  constructor
   · rfl
   · unfold SemanticTyping at ht
-    sorry
+    intro arg harg
+    simp [Exp.from_TypeEnv_weaken_open]
+    apply ht
+    constructor
+    { exact harg }
+    { exact hts }
+
+theorem sem_typ_tabs
+  (ht : (Γ,X<:S) ⊨ e : T) :
+  Γ ⊨ (.tabs S e) : (.poly S T) := by
+  intro env store hts
+  simp [Ty.exp_denot]
+  constructor; constructor
+  apply And.intro Reduce.red_refl _
+  simp [Ty.val_denot]
+  constructor; constructor
+  constructor
+  · rfl
+  · unfold SemanticTyping at ht
+    intro denot hdenot
+    simp [Exp.from_TypeEnv_weaken_open_tvar (d:=denot)]
+    apply ht
+    constructor
+    { exact hdenot }
+    { exact hts }
+
+theorem sem_typ_app
+  (ht1 : Γ ⊨ (.var x) : (.arrow T1 T2))
+  (ht2 : Γ ⊨ (.var y) : T1) :
+  Γ ⊨ (.app x y) : (T2.subst (Subst.openVar x)) := by
+  intro env store hts
+  simp [Ty.exp_denot]
+  unfold SemanticTyping at ht1 ht2
+  simp [Ty.exp_denot, Ty.val_denot] at ht1
+  sorry
 
 theorem soundness
   (ht : Γ ⊢ e : T) :
   Γ ⊨ e : T := by
   induction ht
   case var => apply sem_typ_var
-  case abs => sorry
+  case abs => grind [sem_typ_abs]
+  case tabs => grind [sem_typ_tabs]
+  case app => sorry
   all_goals sorry
 
 end Fsub
